WIP: 2-index RST effect; pointer resource with non-scoped allocation and deallocation

pulse/ulib/LowStar.RST.TwoIndex.fst
@@ -22,20 +22,25 @@ module HST = FStar.HyperStack.ST
 
 open LowStar.Resource
 
-(* Additional (currently assumed) lemma: 
-     Reasonable when addresses are not reused after deallocation, 
-     but currently not provided by the LowStar.Buffer library
-     (Nik and/or Tahina will look into adding it to ulib) *)
-assume val lemma_loc_not_unused_in_modifies_includes (l0 l1:B.loc) (h0 h1:HS.mem)
+(* Additional (currently assumed) lemmas: 
+   [DA: Reasonable when addresses are not reused after deallocation, 
+        but currently was not able to derive them from LowStar's buffers 
+        library (Nik and/or Tahina will look into adding it to buffers library). 
+        There are some other such assumed dotter around the RST development.] *)
+
+assume val lemma_loc_not_unused_in_modifies (l0 l1:B.loc) (h0 h1:HS.mem)
   : Lemma (requires (B.loc_includes (B.loc_not_unused_in h0) l0 /\ 
                      B.loc_includes l1 l0 /\ B.modifies l1 h0 h1))
           (ensures  (B.loc_includes (B.loc_not_unused_in h1) l1))
 
-(* Another (currently assumed) lemma *)
 assume val lemma_modifies_loc_disjoint (l0 l1:B.loc) (h0 h1 h2:HS.mem) 
   : Lemma (requires (B.modifies l0 h0 h1 /\
                      B.modifies l1 h1 h2 /\ 
-                     (forall l . B.loc_disjoint l l0 ==> B.loc_disjoint l l1)))
+                     (forall l . 
+                       B.loc_disjoint l l0 /\ 
+                       B.loc_includes (B.loc_not_unused_in h0) l 
+                       ==> 
+                       B.loc_disjoint l l1)))
           (ensures  (B.modifies l0 h0 h2))
 
 (* Abstract modifies clause for the resource-indexed state effect *)
@@ -43,12 +48,17 @@ assume val lemma_modifies_loc_disjoint (l0 l1:B.loc) (h0 h1 h2:HS.mem)
 abstract
 let modifies (res0 res1:resource) (h0 h1:HS.mem) =
     B.modifies (as_loc (fp res0)) h0 h1 /\ 
-    (forall l . B.loc_disjoint l (as_loc (fp res0)) ==> B.loc_disjoint l (as_loc (fp res1)))
+    (forall frame . 
+      B.loc_disjoint frame (as_loc (fp res0)) /\ 
+      B.loc_includes (B.loc_not_unused_in h0) frame 
+      ==> 
+      B.loc_disjoint frame (as_loc (fp res1)) /\
+      B.loc_includes (B.loc_not_unused_in h1) frame)
 
 let modifies_refl (res:resource) (h:HS.mem) 
   : Lemma (modifies res res h h)
-           [SMTPat (modifies res res h h)]
-  = ()
+           [SMTPat (modifies res res h h)] =
+  ()
 
 let modifies_trans (res0 res1 res2:resource) (h0 h1 h2:HS.mem) 
   : Lemma (requires 
@@ -57,14 +67,19 @@ let modifies_trans (res0 res1 res2:resource) (h0 h1 h2:HS.mem)
            (ensures
              modifies res0 res2 h0 h2)
            [SMTPat (modifies res0 res2 h0 h2);
-            SMTPat (modifies res0 res1 h0 h1)] =
+            SMTPat (modifies res0 res1 h0 h1)] = 
   lemma_modifies_loc_disjoint (as_loc (fp res0)) (as_loc (fp res1)) h0 h1 h2
-
+    
 let reveal_modifies ()
   : Lemma (forall res0 res1 h0 h1.{:pattern modifies res0 res1 h0 h1}
              modifies res0 res1 h0 h1 <==>
              B.modifies (as_loc (fp res0)) h0 h1 /\
-             (forall frame . B.loc_disjoint frame (as_loc (fp res0)) ==> B.loc_disjoint frame (as_loc (fp res1))))
+             (forall frame . 
+               B.loc_disjoint frame (as_loc (fp res0)) /\ 
+               B.loc_includes (B.loc_not_unused_in h0) frame 
+               ==> 
+               B.loc_disjoint frame (as_loc (fp res1)) /\
+               B.loc_includes (B.loc_not_unused_in h1) frame))
   = ()
 
 (* State effect indexed by resources *)
@@ -83,34 +98,32 @@ let reveal_rst_inv ()
              B.loc_includes (B.loc_not_unused_in h) (as_loc (fp res)))
   = ()
 
-let post_resource res0 a =
-  a -> res1:resource{(forall frame . B.loc_disjoint frame (as_loc (fp res0)) ==> B.loc_disjoint frame (as_loc (fp res1)))}
-
-let rst_wp (a:Type) (res0:resource) (res1:post_resource res0 a) = 
+// Monotonic WPs for RSTATE
+let rstate_wp (a:Type) (res0:resource) (res1:a -> resource) = 
   wp:((x:a -> imem (inv (res1 x)) -> Type0) -> imem (inv res0) -> Type0){
       forall (p q:(x:a -> imem (inv (res1 x)) -> Type0)) h0 . (forall x h1 . p x h1 ==> q x h1) ==> wp p h0 ==> wp q h0
     }
 
 effect RSTATE (a:Type)
-              (res0:resource)                                   //Pre-resource (expected from the caller)
-              (res1:post_resource res0 a)                       //Post-resource (returned back to the caller)
-              (wp:rst_wp a res0 res1) =
+              (res0:resource)                                   // Pre-resource (expected from the caller)
+              (res1:a -> resource)                              // Post-resource (returned back to the caller)
+              (wp:rstate_wp a res0 res1) =
        STATE a 
            (fun (p:a -> HS.mem -> Type)
               (h0:HS.mem) -> 
-                inv res0 h0 /\                                  //Require the pre-resource invariant
-                rst_inv res0 h0 /\                              //Require the additional footprints invariant
+                inv res0 h0 /\                                  // Require the pre-resource invariant
+                rst_inv res0 h0 /\                              // Require the additional footprints invariant
                 wp (fun x h1 -> 
-                     inv (res1 x) h1 /\                         //Ensure the post-resource invariant
-                     rst_inv (res1 x) h1 /\                     //Ensure the additional footprints invariant
-                     modifies res0 (res1 x) h0 h1 ==>           //Ensure that at most resources' footprints are modified
-                     p x h1) h0)                                //Prove the continuation under this hypothesis
+                     inv (res1 x) h1 /\                         // Ensure the post-resource invariant
+                     rst_inv (res1 x) h1 /\                     // Ensure the additional footprints invariant
+                     modifies res0 (res1 x) h0 h1 ==>           // Ensure that at most resources' footprints are modified
+                     p x h1) h0)                                // Prove the continuation under this hypothesis
 
 (* Pre- and postcondition style effect RST *)
 
 effect RST (a:Type)
            (res0:resource)
-           (res1:post_resource res0 a)
+           (res1:a -> resource)
            (pre:r_pre res0)
            (post:r_post res0 a res1) = 
        RSTATE a res0 res1 (fun p h0 -> 
@@ -120,12 +133,10 @@ effect RST (a:Type)
 
 let bind (#a #b:Type)
          (#res0:resource)
-         (#res1:post_resource res0 a)
-         (#res2:(b -> res2:resource{(forall frame x . B.loc_disjoint frame (as_loc (fp (res1 x))) ==> B.loc_disjoint frame (as_loc (fp (res2)))) /\
-                                    // only provable from other refinements if we know that a is inhabited
-                                    (forall frame . B.loc_disjoint frame (as_loc (fp res0)) ==> B.loc_disjoint frame (as_loc (fp res2)))}))
-         (#wp0:rst_wp a res0 res1)
-         (#wp1:(x:a -> rst_wp b (res1 x) res2))
+         (#res1:a -> resource)
+         (#res2:b -> resource)
+         (#wp0:rstate_wp a res0 res1)
+         (#wp1:(x:a -> rstate_wp b (res1 x) res2))
          (f:unit -> RSTATE a res0 res1 wp0)
          (g:(x:a -> RSTATE b (res1 x) res2 (wp1 x)))
        : RSTATE b res0 res2 (fun p h0 -> wp0 (fun x h1 -> wp1 x p h1) h0) = 
@@ -138,19 +149,19 @@ let frame_post_delta (#outer0:resource)
                      (#inner0:resource)
                      (delta0:r_includes outer0 inner0)
                      (a:Type)
-                     (outer1:post_resource outer0 a)
-                     (inner1:post_resource inner0 a) =
+                     (outer1:a -> resource)
+                     (inner1:a -> resource) =
   x:a -> delta1:r_includes (outer1 x) (inner1 x){delta0 == delta1}
 
 let frame_wp (#outer0:resource)
           (#inner0:resource)
           (#a:Type)
-          (#outer1:post_resource outer0 a)
-          (#inner1:post_resource inner0 a)
+          (#outer1:a -> resource)
+          (#inner1:a -> resource)
           (delta0:r_includes outer0 inner0)
           (delta1:frame_post_delta delta0 a outer1 inner1)
-          (wp:rst_wp a inner0 inner1)
-        : rst_wp a outer0 outer1 =
+          (wp:rstate_wp a inner0 inner1)
+        : rstate_wp a outer0 outer1 =
   fun p h0 -> 
     wp (fun x (h1:imem (inv (inner1 x))) -> 
           inv (delta1 x) h1 /\ 
@@ -161,23 +172,16 @@ let frame_wp (#outer0:resource)
 let frame (#outer0:resource)
           (#inner0:resource)
           (#a:Type)
-          (#outer1:post_resource outer0 a)
-          (#inner1:post_resource inner0 a)
+          (#outer1:a -> resource)
+          (#inner1:a -> resource)
           (delta0:r_includes outer0 inner0)
           (delta1:frame_post_delta delta0 a outer1 inner1)
-          (#wp:rst_wp a inner0 inner1)
+          (#wp:rstate_wp a inner0 inner1)
           ($f:unit -> RSTATE a inner0 inner1 wp)
         : RSTATE a outer0 outer1 (frame_wp delta0 delta1 wp) =
   reveal_view ();
-  let h0 = get () in 
-  let x = f () in 
-  let h1 = get () in 
-  lemma_loc_not_unused_in_modifies_includes 
-    (as_loc (fp outer0)) 
-    (as_loc (fp (r_union outer0 (outer1 x)))) 
-    h0 h1;
-  x
-
+  f ()
+  
 (* Generic framing operation for RST (through resource inclusion) *)
 
 unfold
@@ -192,8 +196,8 @@ unfold
 let frame_post (#outer0:resource)
                (#inner0:resource)
                (#a:Type)
-               (#outer1:post_resource outer0 a)
-               (#inner1:post_resource inner0 a)
+               (#outer1:a -> resource)
+               (#inner1:a -> resource)
                (delta0:r_includes outer0 inner0)
                (delta1:frame_post_delta delta0 a outer1 inner1)
                (post:r_post inner0 a inner1)
@@ -209,8 +213,8 @@ let frame_post (#outer0:resource)
 let rst_frame (#outer0:resource)
               (#inner0:resource)
               (#a:Type)
-              (#outer1:post_resource outer0 a)
-              (#inner1:post_resource inner0 a)
+              (#outer1:a -> resource)
+              (#inner1:a -> resource)
               (delta0:r_includes outer0 inner0)
               (delta1:frame_post_delta delta0 a outer1 inner1)
               (#pre:r_pre inner0)
@@ -220,13 +224,6 @@ let rst_frame (#outer0:resource)
                     (frame_pre delta0 pre) 
                     (frame_post delta0 delta1 post) =
   reveal_view ();
-  let h0 = get () in 
   let x = f () in 
-  let h1 = get () in 
   assert (delta0 == delta1 x); // here to trigger the refinement on (delta1 x)
-  lemma_loc_not_unused_in_modifies_includes 
-    (as_loc (fp outer0)) 
-    (as_loc (fp (r_union outer0 (outer1 x)))) 
-    h0 h1;
   x
-
